Props/RingSubmitter: prove the fact that subrings are disallowed

Props/RingSubmitterProps.v
@@ -9,10 +9,427 @@ Require Import
         States
         Types.
 Require Import
-        BrokerInterceptor
-        BrokerRegistry
-        ERC20
-        FeeHolder
-        OrderRegistry
-        RingSubmitter
-        TradeDelegate.
+        RingSubmitter.
+Require Import
+        TopModel.
+
+
+Section NoSubRings.
+
+  Definition has_subrings
+             (rings: list RingSubmitter.RingRuntimeState)
+             (orders: list RingSubmitter.OrderRuntimeState) : Prop :=
+    forall r rs,
+      rings = r :: rs /\ RingSubmitter.ring_has_subrings r orders.
+
+  Theorem no_sub_rings:
+    forall sender r orders mining st wst wst' retval events,
+      st = RingSubmitter.make_rt_submitter_state mining orders (r :: nil) ->
+      has_subrings (RingSubmitter.submitter_rt_rings st)
+                   (RingSubmitter.submitter_rt_orders st) ->
+      lr_step wst
+              (MsgRingSubmitter (msg_submitRings sender orders (r :: nil) mining))
+              wst' retval events ->
+      In (EvtRingSkipped r) events.
+  Proof.
+    intros until events.
+    intros Hst Hsubring Hstep.
+
+    simpl in Hstep.
+    unfold RingSubmitter.model in Hstep.
+    destruct Hstep as [_ [st' Hstep]].
+    specialize (Hstep sender orders (r :: nil) mining).
+    destruct Hstep as [_ Hstep].
+
+    assert (Hsubrings0:
+              RingSubmitter.nth_ring_has_subrings (RingSubmitter.make_rt_ring r :: nil)
+                                                  (RingSubmitter.make_rt_orders orders) 0).
+    {
+      rewrite Hst in Hsubring; simpl in Hsubring.
+      specialize (Hsubring (RingSubmitter.make_rt_ring r) nil).
+      destruct Hsubring as [_ Hsubring].
+
+      unfold RingSubmitter.nth_ring_has_subrings; simpl.
+      intros r0 Hnth0; inversion Hnth0; subst.
+
+      trivial.
+    }
+
+    inversion Hstep; clear Hstep; subst.
+    assert (Hsubrings1: RingSubmitter.nth_ring_has_subrings
+                          (RingSubmitter.submitter_rt_rings st'0)
+                          (RingSubmitter.submitter_rt_orders st'0)
+                          0).
+    {
+      inversion H6; clear H6; subst.
+      clear H0 H9; simpl in H1.
+      destruct H1 as [_ [_ Hst_preserve]].
+      destruct Hst_preserve as [Hrings_preserve Hsubrings_preserve].
+      unfold RingSubmitter.subrings_preserve in Hsubrings_preserve;
+        simpl in Hsubrings_preserve.
+      apply Hsubrings_preserve; auto.
+    }
+    assert (Hring1:
+              exists r1,
+                nth_error (RingSubmitter.submitter_rt_rings st'0) 0 = Some r1 /\
+                RingSubmitter.ring_rt_static r1 = r).
+    {
+      inversion H6; clear H6; subst.
+      clear H0 H9; simpl in H1.
+      destruct H1 as [_ [_ Hst_preserve]].
+      destruct Hst_preserve as [Hrings_preserve _].
+      specialize (Hrings_preserve 0).
+      destruct Hrings_preserve as [Hrings_preserve _];
+        simpl in Hrings_preserve.
+      specialize (Hrings_preserve (RingSubmitter.make_rt_ring r));
+        simpl in Hrings_preserve.
+      apply Hrings_preserve; trivial.
+    }
+
+    inversion H7; clear H7; subst.
+    assert (Hsubrings2: RingSubmitter.nth_ring_has_subrings
+                          (RingSubmitter.submitter_rt_rings st'1)
+                          (RingSubmitter.submitter_rt_orders st'1)
+                          0).
+    {
+      inversion H8; clear H8; subst.
+      clear H0 H10; simpl in H1.
+      destruct H1 as [Hst_preserve _].
+      destruct Hst_preserve as [Hrings_preserve Hsubrings_preserve].
+      unfold RingSubmitter.subrings_preserve in Hsubrings_preserve;
+        simpl in Hsubrings_preserve.
+      apply Hsubrings_preserve; auto.
+    }
+    assert (Hring2:
+              exists r2,
+                nth_error (RingSubmitter.submitter_rt_rings st'1) 0 = Some r2 /\
+                RingSubmitter.ring_rt_static r2 = r).
+    {
+      inversion H8; clear H8; subst.
+      clear H0 H10; simpl in H1.
+      destruct H1 as [Hst_preserve _].
+      destruct Hst_preserve as [Hrings_preserve _].
+      specialize (Hrings_preserve 0).
+      destruct Hrings_preserve as [Hrings_preserve _].
+
+      destruct Hring1 as [r1 [Hnth1 Hring1]].
+      specialize (Hrings_preserve r1 Hnth1).
+      destruct Hrings_preserve as [r' [Hnth' Hring']].
+
+      exists r'. split; congruence.
+    }
+
+    inversion H9; clear H9; subst.
+    assert (Hsubrings3: RingSubmitter.nth_ring_has_subrings
+                          (RingSubmitter.submitter_rt_rings st'2)
+                          (RingSubmitter.submitter_rt_orders st'2)
+                          0).
+    {
+      inversion H7; clear H7; subst.
+      clear H0 H11; simpl in H1.
+      destruct H1 as [Hst_preserve _].
+      destruct Hst_preserve as [Hrings_preserve Hsubrings_preserve].
+      unfold RingSubmitter.subrings_preserve in Hsubrings_preserve;
+        simpl in Hsubrings_preserve.
+      apply Hsubrings_preserve; auto.
+    }
+    assert (Hring3:
+              exists r3,
+                nth_error (RingSubmitter.submitter_rt_rings st'2) 0 = Some r3 /\
+                RingSubmitter.ring_rt_static r3 = r).
+    {
+      inversion H7; clear H7; subst.
+      clear H0 H11; simpl in H1.
+      destruct H1 as [Hst_preserve _].
+      destruct Hst_preserve as [Hrings_preserve _].
+      specialize (Hrings_preserve 0).
+      destruct Hrings_preserve as [Hrings_preserve _].
+
+      destruct Hring2 as [r2 [Hnth2 Hring2]].
+      specialize (Hrings_preserve r2 Hnth2).
+      destruct Hrings_preserve as [r' [Hnth' Hring']].
+
+      exists r'. split; congruence.
+    }
+
+    inversion H10; clear H10; subst.
+    assert (Hsubrings4: RingSubmitter.nth_ring_has_subrings
+                          (RingSubmitter.submitter_rt_rings st'3)
+                          (RingSubmitter.submitter_rt_orders st'3)
+                          0).
+    {
+      inversion H9; clear H9; subst.
+      clear H0 H11; simpl in H1.
+      destruct H1 as [_ [Hst_preserve _]].
+      destruct Hst_preserve as [Hrings_preserve Hsubrings_preserve].
+      unfold RingSubmitter.subrings_preserve in Hsubrings_preserve;
+        simpl in Hsubrings_preserve.
+      apply Hsubrings_preserve; auto.
+    }
+    assert (Hring4:
+              exists r4,
+                nth_error (RingSubmitter.submitter_rt_rings st'3) 0 = Some r4 /\
+                RingSubmitter.ring_rt_static r4 = r).
+    {
+      inversion H9; clear H9; subst.
+      clear H0 H11; simpl in H1.
+      destruct H1 as [_ [Hst_preserve _]].
+      destruct Hst_preserve as [Hrings_preserve _].
+      specialize (Hrings_preserve 0).
+      destruct Hrings_preserve as [Hrings_preserve _].
+
+      destruct Hring3 as [r3 [Hnth3 Hring3]].
+      specialize (Hrings_preserve r3 Hnth3).
+      destruct Hrings_preserve as [r' [Hnth' Hring']].
+
+      exists r'. split; congruence.
+    }
+
+    inversion H11; clear H11; subst.
+    assert (Hsubrings5: RingSubmitter.nth_ring_has_subrings
+                          (RingSubmitter.submitter_rt_rings st'4)
+                          (RingSubmitter.submitter_rt_orders st'4)
+                          0).
+    {
+      inversion H10; clear H10; subst.
+      clear H0 H13; simpl in H1.
+      destruct H1 as [_ [_ Hst_preserve]].
+      destruct Hst_preserve as [Hrings_preserve Hsubrings_preserve].
+      unfold RingSubmitter.subrings_preserve in Hsubrings_preserve;
+        simpl in Hsubrings_preserve.
+      apply Hsubrings_preserve; auto.
+    }
+    assert (Hring5:
+              exists r5,
+                nth_error (RingSubmitter.submitter_rt_rings st'4) 0 = Some r5 /\
+                RingSubmitter.ring_rt_static r5 = r).
+    {
+      inversion H10; clear H10; subst.
+      clear H0 H13; simpl in H1.
+      destruct H1 as [_ [_ Hst_preserve]].
+      destruct Hst_preserve as [Hrings_preserve _].
+      specialize (Hrings_preserve 0).
+      destruct Hrings_preserve as [Hrings_preserve _].
+
+      destruct Hring4 as [r4 [Hnth4 Hring4]].
+      specialize (Hrings_preserve r4 Hnth4).
+      destruct Hrings_preserve as [r' [Hnth' Hring']].
+
+      exists r'. split; congruence.
+    }
+
+    inversion H12; clear H12; subst.
+    assert (Hsubrings6: RingSubmitter.nth_ring_has_subrings
+                          (RingSubmitter.submitter_rt_rings st'5)
+                          (RingSubmitter.submitter_rt_orders st'5)
+                          0).
+    {
+      inversion H11; clear H11; subst.
+      clear H0 H14; simpl in H1.
+      destruct H1 as [_ [_ Hst_preserve]].
+      destruct Hst_preserve as [Hrings_preserve Hsubrings_preserve].
+      unfold RingSubmitter.subrings_preserve in Hsubrings_preserve;
+        simpl in Hsubrings_preserve.
+      apply Hsubrings_preserve; auto.
+    }
+    assert (Hring6:
+              exists r6,
+                nth_error (RingSubmitter.submitter_rt_rings st'5) 0 = Some r6 /\
+                RingSubmitter.ring_rt_static r6 = r).
+    {
+      inversion H11; clear H11; subst.
+      clear H0 H14; simpl in H1.
+      destruct H1 as [_ [_ Hst_preserve]].
+      destruct Hst_preserve as [Hrings_preserve _].
+      specialize (Hrings_preserve 0).
+      destruct Hrings_preserve as [Hrings_preserve _].
+
+      destruct Hring5 as [r5 [Hnth5 Hring5]].
+      specialize (Hrings_preserve r5 Hnth5).
+      destruct Hrings_preserve as [r' [Hnth' Hring']].
+
+      exists r'. split; congruence.
+    }
+
+    inversion H13; clear H13; subst.
+    assert (Hsubrings7: RingSubmitter.nth_ring_has_subrings
+                          (RingSubmitter.submitter_rt_rings st'6)
+                          (RingSubmitter.submitter_rt_orders st'6)
+                          0).
+    {
+      inversion H12; clear H12; subst.
+      clear H0 H15; simpl in H1.
+      destruct H1 as [_ [_ Hst_preserve]].
+      destruct Hst_preserve as [Hrings_preserve Hsubrings_preserve].
+      unfold RingSubmitter.subrings_preserve in Hsubrings_preserve;
+        simpl in Hsubrings_preserve.
+      apply Hsubrings_preserve; auto.
+    }
+    assert (Hring7:
+              exists r',
+                nth_error (RingSubmitter.submitter_rt_rings st'6) 0 = Some r' /\
+                RingSubmitter.ring_rt_static r' = r).
+    {
+      inversion H12; clear H12; subst.
+      clear H0 H15; simpl in H1.
+      destruct H1 as [_ [_ Hst_preserve]].
+      destruct Hst_preserve as [Hrings_preserve Hsubrings_preserve].
+
+      specialize (Hrings_preserve 0).
+      destruct Hrings_preserve as [Hrings_preserve _].
+
+      destruct Hring6 as [r'' [Hnth'' Hring'']].
+      specialize (Hrings_preserve r'' Hnth'').
+      destruct Hrings_preserve as [r' [Hnth' Hring']].
+
+      exists r'. split; congruence.
+    }
+
+    inversion H14; clear H14; subst.
+    assert (Hsubrings8: RingSubmitter.nth_ring_has_subrings
+                          (RingSubmitter.submitter_rt_rings st'7)
+                          (RingSubmitter.submitter_rt_orders st'7)
+                          0).
+    {
+      inversion H13; clear H13; subst.
+      clear H0 H16; simpl in H1.
+      destruct H1 as [_ [_ Hst_preserve]].
+      destruct Hst_preserve as [Hrings_preserve Hsubrings_preserve].
+      unfold RingSubmitter.subrings_preserve in Hsubrings_preserve;
+        simpl in Hsubrings_preserve.
+      apply Hsubrings_preserve; auto.
+    }
+    assert (Hring8:
+              exists r',
+                nth_error (RingSubmitter.submitter_rt_rings st'7) 0 = Some r' /\
+                RingSubmitter.ring_rt_static r' = r).
+    {
+      inversion H13; clear H13; subst.
+      clear H0 H16; simpl in H1.
+      destruct H1 as [_ [_ Hst_preserve]].
+      destruct Hst_preserve as [Hrings_preserve Hsubrings_preserve].
+
+      specialize (Hrings_preserve 0).
+      destruct Hrings_preserve as [Hrings_preserve _].
+
+      destruct Hring7 as [r'' [Hnth'' Hring'']].
+      specialize (Hrings_preserve r'' Hnth'').
+      destruct Hrings_preserve as [r' [Hnth' Hring']].
+
+      exists r'. split; congruence.
+    }
+
+    inversion H15; clear H15; subst.
+    assert (Hsubrings9: RingSubmitter.nth_ring_has_subrings
+                          (RingSubmitter.submitter_rt_rings st'8)
+                          (RingSubmitter.submitter_rt_orders st'8)
+                          0).
+    {
+      inversion H14; clear H14; subst.
+      clear H0 H17; simpl in H1.
+      destruct H1 as [_ [_ Hst_preserve]].
+      destruct Hst_preserve as [Hrings_preserve Hsubrings_preserve].
+      unfold RingSubmitter.subrings_preserve in Hsubrings_preserve;
+        simpl in Hsubrings_preserve.
+      apply Hsubrings_preserve; auto.
+    }
+    assert (Hring9:
+              exists r',
+                nth_error (RingSubmitter.submitter_rt_rings st'8) 0 = Some r' /\
+                RingSubmitter.ring_rt_static r' = r).
+    {
+      inversion H14; clear H14; subst.
+      clear H0 H17; simpl in H1.
+      destruct H1 as [_ [_ Hst_preserve]].
+      destruct Hst_preserve as [Hrings_preserve Hsubrings_preserve].
+
+      specialize (Hrings_preserve 0).
+      destruct Hrings_preserve as [Hrings_preserve _].
+
+      destruct Hring8 as [r'' [Hnth'' Hring'']].
+      specialize (Hrings_preserve r'' Hnth'').
+      destruct Hrings_preserve as [r' [Hnth' Hring']].
+
+      exists r'. split; congruence.
+    }
+
+    inversion H16; clear H16; subst.
+    assert (Hsubrings10: RingSubmitter.nth_ring_has_subrings
+                           (RingSubmitter.submitter_rt_rings st'9)
+                           (RingSubmitter.submitter_rt_orders st'9)
+                           0).
+    {
+      inversion H15; clear H15; subst.
+      clear H0 H18; simpl in H1.
+      destruct H1 as [Hst_preserve _].
+      destruct Hst_preserve as [Hrings_preserve Hsubrings_preserve].
+      unfold RingSubmitter.subrings_preserve in Hsubrings_preserve;
+        simpl in Hsubrings_preserve.
+      apply Hsubrings_preserve; auto.
+    }
+    assert (Hring10:
+              exists r',
+                nth_error (RingSubmitter.submitter_rt_rings st'9) 0 = Some r' /\
+                RingSubmitter.ring_rt_static r' = r).
+    {
+      inversion H15; clear H15; subst.
+      clear H0 H18; simpl in H1.
+      destruct H1 as [Hst_preserve _].
+      destruct Hst_preserve as [Hrings_preserve Hsubrings_preserve].
+
+      specialize (Hrings_preserve 0).
+      destruct Hrings_preserve as [Hrings_preserve _].
+
+      destruct Hring9 as [r'' [Hnth'' Hring'']].
+      specialize (Hrings_preserve r'' Hnth'').
+      destruct Hrings_preserve as [r' [Hnth' Hring']].
+
+      exists r'. split; congruence.
+    }
+
+    inversion H17; clear H17; subst.
+    assert (Hsubrings11: RingSubmitter.nth_ring_has_subrings
+                           (RingSubmitter.submitter_rt_rings st'10)
+                           (RingSubmitter.submitter_rt_orders st'10)
+                           0).
+    {
+      inversion H16; clear H16; subst.
+      clear H0 H19; simpl in H1.
+      destruct H1 as [_ [_ Hst_preserve]].
+      destruct Hst_preserve as [Hrings_preserve Hsubrings_preserve].
+      unfold RingSubmitter.subrings_preserve in Hsubrings_preserve;
+        simpl in Hsubrings_preserve.
+      apply Hsubrings_preserve; auto.
+    }
+    assert (Hring11:
+              exists r',
+                nth_error (RingSubmitter.submitter_rt_rings st'10) 0 = Some r' /\
+                RingSubmitter.ring_rt_static r' = r).
+    {
+      inversion H16; clear H16; subst.
+      clear H0 H19; simpl in H1.
+      destruct H1 as [_ [_ Hst_preserve]].
+      destruct Hst_preserve as [Hrings_preserve Hsubrings_preserve].
+
+      specialize (Hrings_preserve 0).
+      destruct Hrings_preserve as [Hrings_preserve _].
+
+      destruct Hring10 as [r'' [Hnth'' Hring'']].
+      specialize (Hrings_preserve r'' Hnth'').
+      destruct Hrings_preserve as [r' [Hnth' Hring']].
+
+      exists r'. split; congruence.
+    }
+
+    inversion H18; clear H18; subst.
+    clear H0 H1; simpl in H19.
+    destruct H19 as [Hring_skipped _].
+
+    destruct Hring11 as [r' [Hnth11 Hring11]].
+    specialize (Hring_skipped 0 r' Hsubrings11 Hnth11).
+    rewrite Hring11 in Hring_skipped.
+
+    repeat (apply in_or_app; right); auto.
+  Qed.
+
+End NoSubRings.
